

Assignment - 3, QFT  
 TOPIC:- ALGEBRAIC STRUCTURES IN QFT  
 Solved by- Pujal Mandal

Q.1) The Weyl representation of gamma matrices is given by

$$\gamma^0 = \begin{pmatrix} 0 & 1 \\ 1 & 0 \end{pmatrix} \quad \gamma^i = \begin{pmatrix} 0 & \sigma^i \\ -\sigma^i & 0 \end{pmatrix}$$

$$i = 1, 2, 3$$

where  $\sigma^i$  are the pauli matrices and 1 denotes  $2 \times 2$  Identity matrix.

Show that these matrices satisfy the Clifford Algebra,  
 $\{\gamma^\mu, \gamma^\nu\} = 2\eta^{\mu\nu}$

Solution:-

$$\gamma^0 = \begin{pmatrix} 0 & 1 \\ 1 & 0 \end{pmatrix}, \gamma^i = \begin{pmatrix} 0 & \sigma^i \\ -\sigma^i & 0 \end{pmatrix} \quad i = 1, 2, 3$$

we know that pauli matrices satisfy

$$\{\sigma^i, \sigma^j\} = 2\delta^{ij} \mathbb{I}_{2 \times 2}$$

$$\Rightarrow \{\gamma^0, \gamma^0\} = (\gamma^0)^2 = 2 \begin{pmatrix} 1 & 0 \\ 0 & 1 \end{pmatrix} = 1_{4 \times 4} \\ = 2 \mathbb{I}_{4 \times 4} = 2\eta^{00} \mathbb{I}$$

$$\Rightarrow \{\gamma^0, \gamma^i\} = \gamma^0 \gamma^i + \gamma^i \gamma^0 \\ = \begin{pmatrix} -\sigma^i & 0 \\ 0 & \sigma^i \end{pmatrix} + \begin{pmatrix} \sigma^i & 0 \\ 0 & -\sigma^i \end{pmatrix} \\ = \begin{pmatrix} 0 & 0 \\ 0 & 0 \end{pmatrix} = 0 = 2\eta^{0i} \mathbb{I}$$

$$\Rightarrow \{\gamma^i, \gamma^j\} = \gamma^i \gamma^j + \gamma^j \gamma^i = - \begin{pmatrix} \sigma^i \sigma^j + \sigma^j \sigma^i & 0 \\ 0 & \sigma^i \sigma^j + \sigma^j \sigma^i \end{pmatrix} \\ = - \begin{pmatrix} \{\sigma^i, \sigma^j\} & 0 \\ 0 & \{\sigma^i, \sigma^j\} \end{pmatrix}$$

$$\{\gamma^i, \gamma^j\} = -2\delta^{ij}I = 2\eta^{ij}I$$

hence,

$$\boxed{\{\gamma^\mu, \gamma^\nu\} = 2\eta^{\mu\nu} I_{4 \times 4}}$$

Hence the Weyl Gamma matrices satisfy the Clifford algebra

Q.2. Assume gamma matrices satisfy the Clifford algebra

$$\{\gamma^\mu, \gamma^\nu\} = 2\eta^{\mu\nu}$$

show that a)  $\text{Tr}(\gamma^\mu) = 0$

b)  $\text{Tr}(\gamma^\mu \gamma^\nu) = 4\eta^{\mu\nu}$

c)  $\text{Tr}(\gamma^\mu \gamma^\nu \gamma^\rho) = 0$

Solution: - As we have assumed  $\gamma \rightarrow$  satisfies Clifford algebra

b)  $\{\gamma^\mu, \gamma^\nu\} = \gamma^\mu \gamma^\nu + \gamma^\nu \gamma^\mu = 2\eta^{\mu\nu} 1$

taking traces of both side  $\rightarrow$

$$\Rightarrow \text{Tr}(\gamma^\mu \gamma^\nu) + \text{Tr}(\gamma^\nu \gamma^\mu) = 2\eta^{\mu\nu} \text{Tr}(I)$$

$$\Rightarrow 2\text{Tr}(\gamma^\mu \gamma^\nu) = 2\eta^{\mu\nu} \text{Tr}(I) \quad [\because \text{Tr}(\gamma^\mu \gamma^\nu) = \text{Tr}(\gamma^\nu \gamma^\mu)]$$

$$\Rightarrow \text{Tr}(\gamma^\mu \gamma^\nu) = \eta^{\mu\nu} \text{Tr}(I) \quad [\because \text{Tr}(I)_{4 \times 4} = 4]$$

$$\Rightarrow \boxed{\text{Tr}(\gamma^\mu \gamma^\nu) = 4\eta^{\mu\nu}}$$

a)  $\gamma^\nu \gamma^\mu = -\gamma^\mu \gamma^\nu \rightarrow$  from Clifford algebra

multiply by  $\gamma^\nu$  on right

$$\gamma^\nu \gamma^\mu \gamma^\nu = -\gamma^\mu (\gamma^\nu)^2$$

$$[\because (\gamma^\nu)^2 = \eta^{\nu\nu} I]$$

$$\Rightarrow \gamma^\mu = -\eta^{\nu\nu} \gamma^\nu \gamma^\mu \gamma^\nu$$

taking trace on both side,

③

$$\text{Tr}(\gamma^\mu) = -\eta^{\nu\nu} \text{Tr}(\gamma^\nu \gamma^\mu \gamma^\nu)$$

$$\text{Tr}(\gamma^\mu) = -\text{Tr}(\gamma^\mu)$$

[using cyclicity  $\rightarrow$   
 $\text{Tr}(\gamma^\nu \gamma^\mu \gamma^\nu) = \text{Tr}(\gamma^\mu (\gamma^\nu)^2)$   
 $= \text{Tr}(\gamma^\mu) \times \eta^{\nu\nu}$ ]

$$\text{Tr}(\gamma^\mu) = -\text{Tr}(\gamma^\mu)$$

$$\Rightarrow \boxed{\text{Tr}(\gamma^\mu) = 0}$$

e) from Clifford algebra

$$\gamma^\mu \gamma^\nu = 2\eta^{\mu\nu} - \gamma^\nu \gamma^\mu$$

multiplying by  $\gamma^\rho \rightarrow$

$$\gamma^\mu \gamma^\nu \gamma^\rho = 2\eta^{\mu\nu} \gamma^\rho - \gamma^\nu \gamma^\mu \gamma^\rho$$

Taking Trace,

$$\text{Tr}(\gamma^\mu \gamma^\nu \gamma^\rho) = 2\eta^{\mu\nu} \text{Tr}(\gamma^\rho) - \text{Tr}(\gamma^\nu \gamma^\mu \gamma^\rho)$$

from part ②  $\rightarrow \text{Tr}(\gamma^\rho) = 0$

hence,  $\text{Tr}(\gamma^\mu \gamma^\nu \gamma^\rho) = -\text{Tr}(\gamma^\nu \gamma^\mu \gamma^\rho)$  — ①

using cyclicity,  $[\nu \leftrightarrow \mu] \quad [\nu \leftrightarrow \rho]$

$$\text{Tr}(\gamma^\mu \gamma^\nu \gamma^\rho) = \pm \text{Tr}(\gamma^\mu \gamma^\rho \gamma^\nu)$$
 — ②

now  $\gamma^\rho \gamma^\nu = -\gamma^\nu \gamma^\rho + 2\eta^{\rho\nu}$

so multiplying with  $\gamma^\mu$  and taking trace

$$\text{Tr}(\gamma^\mu \gamma^\rho \gamma^\nu) = -\text{Tr}(\gamma^\mu \gamma^\nu \gamma^\rho)$$

Substituting in eq ②, RHS  $\rightarrow$

$$\text{Tr}(\gamma^\mu \gamma^\nu \gamma^\rho) = -\text{Tr}(\gamma^\mu \gamma^\nu \gamma^\rho)$$

$$\text{Tr}(\gamma^\mu \gamma^\nu \gamma^\rho) = 0$$

Q.3. i) Show that if  $\{\gamma^\mu, \gamma^\nu\} = 2\eta^{\mu\nu}$  then

$$[\gamma^\kappa \gamma^\lambda, \gamma^\mu \gamma^\nu] = 2\eta^{\lambda\mu} \gamma^\kappa \gamma^\nu - 2\eta^{\kappa\mu} \gamma^\lambda \gamma^\nu + 2\eta^{\lambda\nu} \gamma^\mu \gamma^\kappa - 2\eta^{\kappa\nu} \gamma^\mu \gamma^\lambda$$

ii) Show further that  $S^{\mu\nu} = \frac{1}{4} [\gamma^\mu, \gamma^\nu] = \frac{1}{2} (\gamma^\mu \gamma^\nu - \gamma^\nu \gamma^\mu)$

Use this to confirm that the matrices  $S^{\mu\nu}$  form a representation of the Lie algebra of Lorentz group.

Solution:-

i) given  $\{\gamma^\mu, \gamma^\nu\} = 2\eta^{\mu\nu}$  — (1)

$$[\gamma^\kappa \gamma^\lambda, \gamma^\mu \gamma^\nu] = \gamma^\kappa \gamma^\lambda \gamma^\mu \gamma^\nu - \gamma^\mu \gamma^\nu \gamma^\kappa \gamma^\lambda$$
 — (2)

reordering 1st product

$$\gamma^\kappa \gamma^\lambda \gamma^\mu \gamma^\nu = \gamma^\kappa (\gamma^\lambda \gamma^\mu) \gamma^\nu$$
 — (3)

now  $\{\gamma^\lambda, \gamma^\mu\} = 2\eta^{\lambda\mu}$

$$\Rightarrow \gamma^\lambda \gamma^\mu = 2\eta^{\lambda\mu} - \gamma^\mu \gamma^\lambda$$

Substituting in (3),  $\gamma^\kappa \gamma^\lambda \gamma^\mu \gamma^\nu = \gamma^\kappa (-\gamma^\mu \gamma^\lambda + 2\eta^{\lambda\mu}) \gamma^\nu$  — (4)

$$= -\gamma^\kappa \gamma^\mu \gamma^\lambda \gamma^\nu + 2\eta^{\lambda\mu} \gamma^\kappa \gamma^\nu$$

reordering second product

$$\gamma^\mu \gamma^\nu \gamma^\kappa \gamma^\lambda = \gamma^\mu (\gamma^\nu \gamma^\kappa) \gamma^\lambda = \gamma^\mu (-\gamma^\kappa \gamma^\nu + 2\eta^{\nu\kappa}) \gamma^\lambda$$
 — (5)
$$= -\gamma^\mu \gamma^\kappa \gamma^\nu \gamma^\lambda + 2\eta^{\nu\kappa} \gamma^\mu \gamma^\lambda$$

now subtracting (5) from (4) →

$$[\gamma^\kappa \gamma^\lambda, \gamma^\mu \gamma^\nu] = -\gamma^\kappa \gamma^\mu \gamma^\lambda \gamma^\nu + 2\eta^{\lambda\mu} \gamma^\kappa \gamma^\nu + \gamma^\mu \gamma^\kappa \gamma^\nu \gamma^\lambda - 2\eta^{\nu\kappa} \gamma^\mu \gamma^\lambda$$
 — (6)

now  $\gamma^\mu \gamma^\kappa \gamma^\nu \gamma^\lambda - \gamma^\kappa \gamma^\mu \gamma^\lambda \gamma^\nu \Rightarrow$  can be reordered

(5)

$$\gamma^\mu \gamma^\kappa \gamma^\nu \gamma^\lambda = \gamma^\mu \gamma^\kappa [-\gamma^\lambda \gamma^\nu + 2\eta^{\nu\lambda}]$$

$$= -\gamma^\mu \gamma^\kappa \gamma^\lambda \gamma^\nu + 2\eta^{\nu\lambda} \gamma^\mu \gamma^\kappa \quad \text{--- (7)}$$

also  $\gamma^\kappa \gamma^\mu \gamma^\lambda \gamma^\nu = (-\gamma^\mu \gamma^\kappa + 2\eta^{\kappa\mu}) \gamma^\lambda \gamma^\nu$

$$= -\gamma^\mu \gamma^\kappa \gamma^\lambda \gamma^\nu + 2\eta^{\kappa\mu} \gamma^\lambda \gamma^\nu \quad \text{--- (8)}$$

So  $\gamma^\mu \gamma^\kappa \gamma^\nu \gamma^\lambda - \gamma^\kappa \gamma^\mu \gamma^\lambda \gamma^\nu$

$$= [-\gamma^\mu \gamma^\kappa \gamma^\lambda \gamma^\nu + 2\eta^{\nu\lambda} \gamma^\mu \gamma^\kappa] + \gamma^\mu \gamma^\kappa \gamma^\lambda \gamma^\nu - 2\eta^{\kappa\mu} \gamma^\lambda \gamma^\nu$$

[using (7) and (8)]

$$= 2\eta^{\nu\lambda} \gamma^\mu \gamma^\kappa - 2\eta^{\kappa\mu} \gamma^\lambda \gamma^\nu$$

now plugging back to eq (6)  $\rightarrow$

$$[\gamma^\kappa \gamma^\lambda, \gamma^\mu \gamma^\nu] = 2\eta^{\lambda\mu} \gamma^\kappa \gamma^\nu - 2\eta^{\nu\kappa} \gamma^\mu \gamma^\lambda - 2\eta^{\kappa\mu} \gamma^\lambda \gamma^\nu + 2\eta^{\nu\lambda} \gamma^\mu \gamma^\kappa \quad \text{--- (9)}$$

i.b) By definition,  $[\gamma^\mu, \gamma^\nu] = \gamma^\mu \gamma^\nu - \gamma^\nu \gamma^\mu \quad \text{--- (10)}$

from (1),  $\gamma^\nu \gamma^\mu = 2\eta^{\mu\nu} - \gamma^\mu \gamma^\nu$

putting in eq (10),  $[\gamma^\mu, \gamma^\nu] = 2(\gamma^\mu \gamma^\nu) - 2\eta^{\mu\nu}$

$$= 2(\gamma^\mu \gamma^\nu - \eta^{\mu\nu})$$

therefore,  $S^{\mu\nu} = \frac{1}{4} [\gamma^\mu, \gamma^\nu] = \frac{1}{2} (\gamma^\mu \gamma^\nu - \eta^{\mu\nu})$



Lorentz Lie Algebra:-

(6)

the Lorentz Lie algebra satisfies,

$$[M^{\mu\nu}, M^{\rho\sigma}] = \eta^{\nu\rho} M^{\mu\sigma} - \eta^{\mu\rho} M^{\nu\sigma} - \eta^{\sigma\mu} M^{\nu\rho} + \eta^{\sigma\nu} M^{\mu\rho} \quad (11)$$

using part (i) and definition of  $S^{\mu\nu} = \frac{1}{4} [\gamma^\mu, \gamma^\nu]$

$$[S^{\kappa\lambda}, S^{\mu\nu}] = \frac{1}{16} [[\gamma^\kappa, \gamma^\lambda], [\gamma^\mu, \gamma^\nu]] \quad (12)$$

$$\text{now } [\gamma^\kappa, \gamma^\lambda] = \gamma^\kappa \gamma^\lambda - \gamma^\lambda \gamma^\kappa$$

$$[\gamma^\mu, \gamma^\nu] = \gamma^\mu \gamma^\nu - \gamma^\nu \gamma^\mu$$

$$[\gamma^\kappa \gamma^\lambda - \gamma^\lambda \gamma^\kappa, \gamma^\mu \gamma^\nu - \gamma^\nu \gamma^\mu]$$

$$= [\gamma^\kappa \gamma^\lambda, \gamma^\mu \gamma^\nu] - [\gamma^\kappa \gamma^\lambda, \gamma^\nu \gamma^\mu] - [\gamma^\lambda \gamma^\kappa, \gamma^\mu \gamma^\nu] + [\gamma^\lambda \gamma^\kappa, \gamma^\nu \gamma^\mu]$$

now using result from i)

$$[\gamma^a \gamma^b, \gamma^c \gamma^d] = 2\eta^{bc} \gamma^a \gamma^d - 2\eta^{ac} \gamma^b \gamma^d + 2\eta^{bd} \gamma^c \gamma^a - 2\eta^{ad} \gamma^c \gamma^b$$

applying this to 1st term,

$$[\gamma^\kappa \gamma^\lambda, \gamma^\mu \gamma^\nu] = 2\eta^{\lambda\mu} \gamma^\kappa \gamma^\nu - 2\eta^{\kappa\mu} \gamma^\lambda \gamma^\nu + 2\eta^{\lambda\nu} \gamma^\kappa \gamma^\mu - 2\eta^{\kappa\nu} \gamma^\lambda \gamma^\mu$$

similarly after applying it to all 4 terms  $\rightarrow$

$$[[\gamma^\kappa, \gamma^\lambda], [\gamma^\mu, \gamma^\nu]] = 8 (\eta^{\lambda\mu} \gamma^\kappa \gamma^\nu - \eta^{\kappa\mu} \gamma^\lambda \gamma^\nu - \eta^{\lambda\nu} \gamma^\kappa \gamma^\mu + \eta^{\kappa\nu} \gamma^\lambda \gamma^\mu)$$

$$[S^{\kappa\lambda}, S^{\mu\nu}] = \frac{1}{16} [[\gamma^\kappa, \gamma^\lambda], [\gamma^\mu, \gamma^\nu]]$$

$$= \frac{8}{16} [\eta^{\lambda\mu} \gamma^\kappa \gamma^\nu - \eta^{\kappa\mu} \gamma^\lambda \gamma^\nu - \eta^{\lambda\nu} \gamma^\kappa \gamma^\mu + \eta^{\kappa\nu} \gamma^\lambda \gamma^\mu] \quad (13)$$

$$\gamma^a \gamma^b = 2S^{ab} + \eta^{ab}$$

$$\text{and } S^{ab} = -S^{ba}$$

$$\Rightarrow \eta^{\lambda\mu} \gamma^{\kappa} \gamma^{\nu} = \eta^{\lambda\mu} (2S^{\kappa\nu} + \eta^{\kappa\nu})$$

$$\Rightarrow -\eta^{\kappa\mu} \gamma^{\lambda} \gamma^{\nu} = -\eta^{\kappa\mu} (2S^{\lambda\nu} + \eta^{\lambda\nu})$$

$$\Rightarrow -\eta^{\lambda\nu} \gamma^{\kappa} \gamma^{\mu} = -\eta^{\lambda\nu} (2S^{\kappa\mu} + \eta^{\kappa\mu})$$

$$\Rightarrow \eta^{\kappa\nu} \gamma^{\lambda} \gamma^{\mu} = \eta^{\kappa\nu} (2S^{\lambda\mu} + \eta^{\lambda\mu})$$

Inserting all these 4 terms back

$$[S^{\kappa\lambda}, S^{\mu\nu}] = \frac{1}{2} [2\eta^{\lambda\mu} S^{\kappa\nu} + \eta^{\lambda\mu} \eta^{\kappa\nu} - 2\eta^{\kappa\mu} S^{\lambda\nu} - \eta^{\kappa\mu} \eta^{\lambda\nu} - 2\eta^{\lambda\nu} S^{\kappa\mu} - \eta^{\lambda\nu} \eta^{\kappa\mu} + 2\eta^{\kappa\nu} S^{\lambda\mu} + \eta^{\kappa\nu} \eta^{\lambda\mu}] \quad (14)$$

$$\text{metric terms} \rightarrow \frac{1}{2} (\eta^{\lambda\mu} \eta^{\kappa\nu} - \eta^{\kappa\mu} \eta^{\lambda\nu} - \eta^{\lambda\nu} \eta^{\kappa\mu} + \eta^{\kappa\nu} \eta^{\lambda\mu})$$

$$\rightarrow \eta^{\lambda\nu} \eta^{\kappa\mu} + \eta^{\kappa\nu} \eta^{\lambda\mu} = 2\eta^{\lambda\mu} \eta^{\kappa\nu} \quad \left. \begin{array}{l} \text{cancels each other} \\ \text{upon adding} \end{array} \right\}$$

$$\rightarrow -\eta^{\kappa\mu} \eta^{\lambda\nu} - \eta^{\lambda\nu} \eta^{\kappa\mu} = -2\eta^{\kappa\mu} \eta^{\lambda\nu}$$

$$[S^{\kappa\lambda}, S^{\mu\nu}] = \frac{1}{2} [2\eta^{\lambda\mu} S^{\kappa\nu} - 2\eta^{\kappa\mu} S^{\lambda\nu} - 2\eta^{\lambda\nu} S^{\kappa\mu} + 2\eta^{\kappa\nu} S^{\lambda\mu}]$$

$$[S^{\kappa\lambda}, S^{\mu\nu}] = \eta^{\lambda\mu} S^{\kappa\nu} - \eta^{\kappa\mu} S^{\lambda\nu} - \eta^{\lambda\nu} S^{\kappa\mu} + \eta^{\kappa\nu} S^{\lambda\mu} \quad (15)$$

And the Lorentz Lie algebra condition,

$$[M^{\mu\nu}, M^{\rho\sigma}] = \eta^{\nu\rho} M^{\mu\sigma} - \eta^{\mu\rho} M^{\nu\sigma} - \eta^{\nu\sigma} M^{\mu\rho} + \eta^{\mu\sigma} M^{\nu\rho} \quad (11)$$

now comparing Eq (15) and Eq (11)  $\rightarrow$  they both

$M^{\mu\nu}$  and  $S^{\mu\nu}$  follows the same condition

hence,  $S^{\mu\nu}$  form a representation of Lie algebra of Lorentz group.